***Absorption:*** 
- $P \wedge P \equiv P$
- $P \wedge P \equiv P$

Commutativity: 
- $P \wedge Q \equiv Q \wedge P$

Associativity:
- $P \wedge (Q \wedge Q) \equiv (P \wedge Q) \wedge Q$
- $P \vee (Q \vee Q) \equiv (P \vee Q) \vee Q$

Distributivity:
- $P \wedge (Q \vee R) \equiv (P \wedge Q) \vee (P \wedge R)$
- $P \vee (Q \wedge R) \equiv (P \vee Q) \wedge (P \vee R)$

Double Negation:
- $P \equiv \neg\neg P$

De Morgan:
- $\neg(P \wedge Q) \equiv \neg P \vee \neg Q$
- $\neg(P \vee Q) \equiv \neg P \wedge \neg Q$

Implication:
- $P \rightarrow Q \equiv \neg P \vee Q$
- $P \rightarrow Q \equiv \neg Q \rightarrow \vee \neg P$


Contraposition:
- $(\neg P \rightarrow \neg Q) \equiv (Q \rightarrow P)$
- $(P \rightarrow \neg Q) \equiv (Q \rightarrow \neg P)$
- $(\neg P \rightarrow  Q) \equiv (\neg Q \rightarrow P)$

Biimplication:
- $P \leftrightarrow Q \equiv (P \wedge Q) \vee (\neg P \wedge \neg Q)$
- $P \leftrightarrow Q \equiv (P \rightarrow Q) \wedge (Q \rightarrow P)$


A $\bigoplus$ B $\equiv$ ($A \vee B$) $\wedge$ ($\neg A \vee \neg B$)


Useful Conversions to CNF:
[[CNF Form#Useful Conversions]]
